changed reactive condition in the program simulation

memabs/ProgSim.v
@@ -1,8 +1,69 @@
+Require Import Relations RelationClasses.
+Require Import List.
 Require Import Integers Coqlib Maps.
 Require Import LanguageInterface Events Globalenvs Values Memory Smallstep.
 Require Import Clight Ctypes Cop.
+Require Import CKLR Clightrel.
 Require Import Coherence CompCertSem Bigstep.
-Require Import SemDef MemAbs.
+Require Import SemDef SepCKLR.
+
+(* A relation that allows arguments in C language interface to be more
+   defined than those in abstract language interface *)
+Inductive q_rel': query li_d -> query li_c -> mem -> Prop:=
+| q_rel'_intro:
+    forall vf sg args args' m,
+      list_rel Val.lessdef args args' ->
+      q_rel' ({|dq_vf:=vf;dq_sg:=sg;dq_args:=args|})
+             ({|cq_vf:=vf;cq_sg:=sg;cq_args:=args';cq_mem:=m|}) m.
+
+Definition r_with_mem (r: reply li_d) m: reply li_c :=
+  match r with
+    {|dr_retval:=ret|} => ({|cr_retval:=ret;cr_mem:=m|})
+  end.
+
+Section REACH.
+  Context {liA liB: language_interface} (Σ: !liA --o !liB).
+  Inductive reachable: !liA --o !liB -> Prop :=
+  | self_reachable: reachable Σ
+  | step_reachable σ q t r:
+      reachable σ -> exec σ q t r ->
+      reachable (next σ t q r).
+End REACH.
+
+Inductive reactive {liA liB: language_interface} (σ: !liA --o !liB) : Prop :=
+| reactive_intro
+    (SPLIT: (forall t q r rest,
+                has σ (t, (q,r) :: rest) ->
+                exists t1 t2, t = t1 ++ t2 /\ exec σ q t1 r))
+    (EMPTY: (forall t, has σ (t, nil) -> t = nil)):
+    reactive σ.
+
+Record prog_sim (p: Clight.program) (Σ: Genv.symtbl -> !li_d --o !li_d) :=
+  {
+  mspec_rel :> (!li_d --o !li_d) -> mem -> Prop;
+  init_mem : mem -> Prop;
+
+  mem_scope : forall m m' σ se,
+      Genv.valid_for (AST.erase_program p) se ->
+      Mem.unchanged_on (module_var (Clight.globalenv se p)) m m' ->
+      mspec_rel σ m ->
+      mspec_rel σ m';
+  simulation: forall σ dq dr t m se cq,
+      Genv.valid_for (AST.erase_program p) se ->
+      mspec_rel σ m -> exec σ dq t dr ->
+      q_rel' dq cq m ->
+      exists m',
+        has (clight_bigstep p se @ !li_dc) (t, (cq, r_with_mem dr m')) /\
+        Mem.unchanged_on (fun b ofs => ~ module_var (Clight.globalenv se p) b ofs) m m' /\
+        (* Mem.unchanged_on allowed non-local variables to grow and we forbid it
+        by adding constraints on Mem.nextblock *)
+        Mem.nextblock m = Mem.nextblock m' /\
+        mspec_rel (next σ t dq dr) m';
+  correct_cond: forall m se,
+      Genv.valid_for (AST.erase_program p) se ->
+      init_mem m -> mspec_rel (Σ se) m;
+  reactive_spec: forall se σ, reachable (Σ se) σ -> reactive σ;
+  }.
 
 Definition q_with_mem (q: query li_d) m: query li_c :=
   match q with
@@ -57,65 +118,65 @@ Proof.
 Qed.
 
 (* Correctness criterion for absfun modules *)
-Section ABSFUN.
-  (* Something weird about the symbol table *)
-  Variable (p: Clight.program) (σ: !li_d --o li_d).
-  Hypothesis sim:
-    forall se, Genv.valid_for (AST.erase_program p) se ->
-          forall t q r m,
-            (* memory extension allows source query to have undefined values so
-               the simulation in prog_sim is strengthened accordingly, which
-               means the verification condition here also has to be augmented *)
-            (* Otherwise, we could changed the calling convention used in the
-               contextual refinement, which might be a better way to work
-               around *)
-            has σ (t, (q, r)) -> query_defined q /\
-            has (clight_bigstep p se @ !li_dc)
-                (t, (q_with_mem q m, r_with_mem r m)).
+(* Section ABSFUN. *)
+(*   (* Something weird about the symbol table *) *)
+(*   Variable (p: Clight.program) (σ: !li_d --o li_d). *)
+(*   Hypothesis sim: *)
+(*     forall se, Genv.valid_for (AST.erase_program p) se -> *)
+(*           forall t q r m, *)
+(*             (* memory extension allows source query to have undefined values so *)
+ (*                the simulation in prog_sim is strengthened accordingly, which *)
+ (*                means the verification condition here also has to be augmented *) *)
+(*             (* Otherwise, we could changed the calling convention used in the *)
+ (*                contextual refinement, which might be a better way to work *)
+ (*                around *) *)
+(*             has σ (t, (q, r)) -> query_defined q /\ *)
+(*             has (clight_bigstep p se @ !li_dc) *)
+(*                 (t, (q_with_mem q m, r_with_mem r m)). *)
 
-  Program Definition psim: prog_sim p (fun se => dag_ext σ) :=
-    {|
-    mspec_rel := fun Σ _ => Σ = dag_ext σ;
-    init_mem := fun _ => True;
-    |}.
-  Next Obligation.
-    exists m. repeat apply conj; try intuition.
-    {
-      inv H1. inv H0. destruct H1. inv H0; inv H1.
-      eapply sim with (m := m) in H6; eauto.
-      destruct H6. eapply defined_query_with_mem in H0; eauto.
-      subst. inv H8. inv H3. rewrite app_nil_r.
-      inv H1. destruct H0.
-      eexists. split.
-      apply H0. apply H1.
-    }
-    {
-      inv H1. inv H0. destruct H1. inv H0; inv H1. inv H8. inv H3.
-      rewrite app_nil_r.
-      apply lmap_ext. intros xs ys.
-      split.
-      - inversion 1. destruct H1. inv H1; inv H3.
-        assert (s = s0).
-        {
-          assert (list_coh _ s0 s).
-          eapply prefix_coh with (t1 := a) (t2 := xs).
-          apply list_coh_refl. apply H4.
-          pose proof (has_coh _ _ _ _ H6 H9).
-          exploit H3. symmetry. apply H1.
-          intros [? ?]. apply H8. auto.
-        }
-        subst. apply app_suffix_eq in H4. subst.
-        eexists. split. apply H5. apply H11.
-      - inversion 1. destruct H1.
-        exists (s :: x). split.
-        constructor. apply H1.
-        constructor. auto. apply H3.
-    }
-  Qed.
-  Next Obligation.
-    constructor.
-    {
-      intros.
+(*   Program Definition psim: prog_sim p (fun se => dag_ext σ) := *)
+(*     {| *)
+(*     mspec_rel := fun Σ _ => Σ = dag_ext σ; *)
+(*     init_mem := fun _ => True; *)
+(*     |}. *)
+(*   Next Obligation. *)
+(*     exists m. repeat apply conj; try intuition. *)
+(*     { *)
+(*       inv H1. inv H0. destruct H1. inv H0; inv H1. *)
+(*       eapply sim with (m := m) in H6; eauto. *)
+(*       destruct H6. eapply defined_query_with_mem in H0; eauto. *)
+(*       subst. inv H8. inv H3. rewrite app_nil_r. *)
+(*       inv H1. destruct H0. *)
+(*       eexists. split. *)
+(*       apply H0. apply H1. *)
+(*     } *)
+(*     { *)
+(*       inv H1. inv H0. destruct H1. inv H0; inv H1. inv H8. inv H3. *)
+(*       rewrite app_nil_r. *)
+(*       apply lmap_ext. intros xs ys. *)
+(*       split. *)
+(*       - inversion 1. destruct H1. inv H1; inv H3. *)
+(*         assert (s = s0). *)
+(*         { *)
+(*           assert (list_coh _ s0 s). *)
+(*           eapply prefix_coh with (t1 := a) (t2 := xs). *)
+(*           apply list_coh_refl. apply H4. *)
+(*           pose proof (has_coh _ _ _ _ H6 H9). *)
+(*           exploit H3. symmetry. apply H1. *)
+(*           intros [? ?]. apply H8. auto. *)
+(*         } *)
+(*         subst. apply app_suffix_eq in H4. subst. *)
+(*         eexists. split. apply H5. apply H11. *)
+(*       - inversion 1. destruct H1. *)
+(*         exists (s :: x). split. *)
+(*         constructor. apply H1. *)
+(*         constructor. auto. apply H3. *)
+(*     } *)
+(*   Qed. *)
+(*   Next Obligation. *)
+(*     constructor. *)
+(*     { *)
+(*       intros. *)
 
-    }
-End ABSFUN.
+(*     } *)
+(* End ABSFUN. *)
